@prefix cms: <http://mu.semte.ch/vocabulary/cms/>.
@prefix foaf: <http://xmlns.com/foaf/0.1/>.
@prefix persoon: <https://data.vlaanderen.be/ns/persoon#>.
@prefix locn: <http://www.w3.org/ns/locn#>.
@prefix schema: <http://schema.org/>.
@prefix adres: <https://data.vlaanderen.be/ns/adres#>.
@prefix person: <http://www.w3.org/ns/person#>.
@prefix ext: <http://mu.semte.ch/vocabularies/ext/>.
@prefix rm: <http://mu.semte.ch/vocabularies/logical-delete/>.
@prefix typedLiterals: <http://mu.semte.ch/vocabularies/typed-literals/>.
@prefix mu: <http://mu.semte.ch/vocabularies/core/>.
@prefix xsd: <http://www.w3.org/2001/XMLSchema#>.
@prefix app: <http://mu.semte.ch/app/>.
@prefix owl: <http://www.w3.org/2002/07/owl#>.
@prefix rdf: <http://www.w3.org/1999/02/22-rdf-syntax-ns#>.
@prefix dc: <http://purl.org/dc/elements/1.1/>.

<http://mu.semte.ch/ontology> rdf:type owl:Ontology.
<http://mu.semte.ch/ontology> dc:title "Generated resource ontology". 
<http://mu.semte.ch/ontology> dc:description "Generated resource ontology". 

person:Person rdf:type owl:Class;
  rdfs:label "person".
adms:Identifier rdf:type owl:Class;
  rdfs:label "identifier".
adres:Adres rdf:type owl:Class;
  rdfs:label "address".
oe:LocatieElementPerceel rdf:type owl:Class;
  rdfs:label "location-parcel".
locn:Address rdf:type owl:Class;
  rdfs:label "address-representation".
schema:ContactPoint rdf:type owl:Class;
  rdfs:label "contact-point".

foaf:familyName rdf:type owl:DatatypeProperty;
  rdfs:comment "Resources type is string.  Original predicate is foaf:familyName.";
  rdfs:label "last-name";
  rdfs:range rdfs:Literal;
  rdfs:domain person:Person.
persoon:gebruikteVoornaam rdf:type owl:DatatypeProperty;
  rdfs:comment "Resources type is string.  Original predicate is persoon:gebruikteVoornaam.";
  rdfs:label "used-first-name";
  rdfs:range rdfs:Literal;
  rdfs:domain person:Person.
skos:notation rdf:type owl:DatatypeProperty;
  rdfs:comment "Resources type is string.  Original predicate is skos:notation.";
  rdfs:label "identifier";
  rdfs:range rdfs:Literal;
  rdfs:domain adms:Identifier.
ext:cadastralDepartment rdf:type owl:DatatypeProperty;
  rdfs:comment "Resources type is string.  Original predicate is ext:cadastralDepartment.";
  rdfs:label "cadastral-department";
  rdfs:range rdfs:Literal;
  rdfs:domain oe:LocatieElementPerceel.
ext:cadastralSection rdf:type owl:DatatypeProperty;
  rdfs:comment "Resources type is string.  Original predicate is ext:cadastralSection.";
  rdfs:label "section";
  rdfs:range rdfs:Literal;
  rdfs:domain oe:LocatieElementPerceel.
ext:cadastralNumber rdf:type owl:DatatypeProperty;
  rdfs:comment "Resources type is string.  Original predicate is ext:cadastralNumber.";
  rdfs:label "number";
  rdfs:range rdfs:Literal;
  rdfs:domain oe:LocatieElementPerceel.
adres:gemeentenaam rdf:type owl:DatatypeProperty;
  rdfs:comment "Resources type is string.  Original predicate is adres:gemeentenaam.";
  rdfs:label "municipality-name";
  rdfs:range rdfs:Literal;
  rdfs:domain locn:Address.
locn:thoroughfare rdf:type owl:DatatypeProperty;
  rdfs:comment "Resources type is string.  Original predicate is locn:thoroughfare.";
  rdfs:label "street-name";
  rdfs:range rdfs:Literal;
  rdfs:domain locn:Address.
locn:postCode rdf:type owl:DatatypeProperty;
  rdfs:comment "Resources type is string.  Original predicate is locn:postCode.";
  rdfs:label "postal-code";
  rdfs:range rdfs:Literal;
  rdfs:domain locn:Address.
adres:Adresvoorstelling.busnummer rdf:type owl:DatatypeProperty;
  rdfs:comment "Resources type is string.  Original predicate is adres:Adresvoorstelling.busnummer.";
  rdfs:label "bus-number";
  rdfs:range rdfs:Literal;
  rdfs:domain locn:Address.
foaf:name rdf:type owl:DatatypeProperty;
  rdfs:comment "Resources type is string.  Original predicate is foaf:name.";
  rdfs:label "name";
  rdfs:range rdfs:Literal;
  rdfs:domain schema:ContactPoint.
schema:email rdf:type owl:DatatypeProperty;
  rdfs:comment "Resources type is string.  Original predicate is schema:email.";
  rdfs:label "email";
  rdfs:range rdfs:Literal;
  rdfs:domain schema:ContactPoint.
schema:telephone rdf:type owl:DatatypeProperty;
  rdfs:comment "Resources type is string.  Original predicate is schema:telephone.";
  rdfs:label "telephone";
  rdfs:range rdfs:Literal;
  rdfs:domain schema:ContactPoint.


schema:contactPoint rdf:type owl:ObjectProperty;
  rdfs:comment "";
  rdfs:label "contact-points";
  rdfs:domain person:Person;
  rdfs:range schema:ContactPoint.
persoon:registratie rdf:type owl:ObjectProperty;
  rdfs:comment "";
  rdfs:label "identifier";
  rdfs:domain person:Person;
  rdfs:range adms:Identifier.
adres:verwijstNaar rdf:type owl:ObjectProperty;
  rdfs:comment "";
  rdfs:label "references";
  rdfs:domain locn:Address;
  rdfs:range adres:Adres.
locn:address rdf:type owl:ObjectProperty;
  rdfs:comment "";
  rdfs:label "address";
  rdfs:domain schema:ContactPoint;
  rdfs:range locn:Address.



